refactor: pull up the call to bitblaster up as much as possible

LeanSAT/Reflect/BVExpr/BitBlast/Impl/Eq.lean
@@ -1,61 +1,29 @@
-import LeanSAT.Reflect.BVExpr.BitBlast.Impl.Expr
+import LeanSAT.AIG
 
 namespace BVPred
 
-def mkEq (aig : AIG BVBit) (pair : ExprPair) : AIG.Entrypoint BVBit :=
-  let res := pair.lhs.bitblast aig
-  let aig := res.aig
-  let lhsRefs := res.stream
-  let res := pair.rhs.bitblast aig
-  let aig := res.aig
-  let rhsRefs := res.stream
-  let lhsRefs := lhsRefs.cast <| by
-    simp (config := { zetaDelta := true }) only
-    apply AIG.LawfulStreamOperator.le_size (f := BVExpr.bitblast)
-  streamProc aig ⟨lhsRefs, rhsRefs⟩
-where
-  streamProc {w : Nat} (aig : AIG BVBit) (input : AIG.BinaryRefStream aig w) : AIG.Entrypoint BVBit :=
-    let res := AIG.RefStream.zip aig ⟨input, AIG.mkBEqCached⟩
-    let aig := res.aig
-    let bits := res.stream
-    AIG.RefStream.fold aig (.mkAnd bits)
+variable [BEq α] [Hashable α] [DecidableEq α]
 
-instance {w : Nat} : AIG.LawfulOperator BVBit (AIG.BinaryRefStream · w) mkEq.streamProc where
+def mkEq (aig : AIG α) (pair : AIG.BinaryRefStream aig w) : AIG.Entrypoint α :=
+  let res := AIG.RefStream.zip aig ⟨pair, AIG.mkBEqCached⟩
+  let aig := res.aig
+  let bits := res.stream
+  AIG.RefStream.fold aig (.mkAnd bits)
+
+instance {w : Nat} : AIG.LawfulOperator α (AIG.BinaryRefStream · w) mkEq where
   le_size := by
     intros
-    unfold mkEq.streamProc
+    unfold mkEq
     dsimp
     apply AIG.LawfulOperator.le_size_of_le_aig_size (f := AIG.RefStream.fold)
     apply AIG.LawfulStreamOperator.le_size (f := AIG.RefStream.zip)
   decl_eq := by
     intros
-    unfold mkEq.streamProc
+    unfold mkEq
     dsimp
     rw [AIG.LawfulOperator.decl_eq (f := AIG.RefStream.fold)]
     rw [AIG.LawfulStreamOperator.decl_eq (f := AIG.RefStream.zip)]
     apply AIG.LawfulStreamOperator.lt_size_of_lt_aig_size (f := AIG.RefStream.zip)
     assumption
-
-instance : AIG.LawfulOperator BVBit (fun _ => ExprPair) mkEq where
-  le_size := by
-    intros
-    unfold mkEq
-    dsimp
-    apply AIG.LawfulOperator.le_size_of_le_aig_size (f := mkEq.streamProc)
-    apply AIG.LawfulStreamOperator.le_size_of_le_aig_size (f := BVExpr.bitblast)
-    apply AIG.LawfulStreamOperator.le_size (f := BVExpr.bitblast)
-  decl_eq := by
-    intros
-    unfold mkEq
-    dsimp
-    rw [AIG.LawfulOperator.decl_eq (f := mkEq.streamProc)]
-    rw [AIG.LawfulStreamOperator.decl_eq (f := BVExpr.bitblast)]
-    rw [AIG.LawfulStreamOperator.decl_eq (f := BVExpr.bitblast)]
-    . apply AIG.LawfulStreamOperator.lt_size_of_lt_aig_size (f := BVExpr.bitblast)
-      assumption
-    . apply AIG.LawfulStreamOperator.lt_size_of_lt_aig_size (f := BVExpr.bitblast)
-      apply AIG.LawfulStreamOperator.lt_size_of_lt_aig_size (f := BVExpr.bitblast)
-      assumption
-
 
 end BVPred
