LeanSAT/Reflect/BVExpr/BitBlast/Lemmas/Pred.lean
@@ -1,6 +1,7 @@
 import LeanSAT.Reflect.BVExpr.BitBlast.Lemmas.Eq
 import LeanSAT.Reflect.BVExpr.BitBlast.Lemmas.Ult
 import LeanSAT.Reflect.BVExpr.BitBlast.Lemmas.GetLsb
+import LeanSAT.Reflect.BVExpr.BitBlast.Lemmas.Expr
 import LeanSAT.Reflect.BVExpr.BitBlast.Impl.Pred
 
 open AIG
@@ -15,9 +16,28 @@ theorem bitblast_denote_eq_eval (aig : AIG BVBit) (pred : BVPred) (assign : BVEx
   cases pred with
   | bin lhs op rhs =>
     cases op with
-    | eq => simp [bitblast]
-    | ult => simp [bitblast]
+    | eq =>
+      simp only [bitblast, eval_bin, BVBinPred.eval_eq]
+      rw [mkEq_denote_eq_eval_beq]
+      . intros
+        rw [AIG.LawfulStreamOperator.denote_mem_prefix (f := BVExpr.bitblast)]
+        . simp
+          rw [BVExpr.bitblast_denote_eq_eval_getLsb]
+        . simp [Ref.hgate]
+      . intros
+        simp
+    | ult =>
+      simp only [bitblast, eval_bin, BVBinPred.eval_ult]
+      rw [mkUlt_denote_eq_eval_ult]
+      . intros
+        rw [AIG.LawfulStreamOperator.denote_mem_prefix (f := BVExpr.bitblast)]
+        . simp
+          rw [BVExpr.bitblast_denote_eq_eval_getLsb]
+        . simp [Ref.hgate]
+      . intros
+        simp
   | getLsb expr idx =>
     simp [bitblast]
+    apply BitVec.lt_of_getLsb
 
 end BVPred
